prove soundness of land and lor.

Solver.v
@@ -2,12 +2,13 @@ Require Import Id Formula.
 From Coq Require Import Lists.ListSet.
 From Coq Require Import Strings.String.
 Import ListNotations.
+Require Setoid. 
 
 
 Definition satisfiable (p : form) : Prop:=
   exists V : valuation, interp V p = true.
 
-Module Test.
+Module Test_satisfiable.
 
  Definition x := (var (Id "x")).
  Definition y := (var (Id "y")).
@@ -25,13 +26,7 @@ Module Test.
    now exists (override (override empty_valuation (Id "x") true) (Id "y") false).
  Qed.
 
-End Test.
-
-
-  
-Check  id_eq_dec.
-
-
+End Test_satisfiable.
 
 Fixpoint collect_var (p : form) : (set id):=
   match p with
@@ -44,7 +39,7 @@ Fixpoint collect_var (p : form) : (set id):=
   end.
 
 
-Module Test'.
+Module Test_collect_var.
 
  Definition x := (var (Id "x")).
  Definition y := (var (Id "y")).
@@ -55,7 +50,7 @@ Eval compute in (collect_var (land (lor x (not y)) (lor (not x) y))).
 
 
 
-End Test'.
+End Test_collect_var.
 
 (*
 Can't defined in the following generator way
@@ -126,7 +121,7 @@ Fixpoint enum_valuation (l : list id) : list valuation :=
   | x::xs => add_id (enum_valuation xs) x
   end.
              
-Module Test''.
+Module Test_enum_valuation.
 
  Definition x := (Id "x").
  Definition y := (Id "y").
@@ -149,7 +144,7 @@ Module Test''.
  Eval compute in (all_valuations (add_id [(override (override empty_valuation x true) y false);(override (override empty_valuation x false) y false);(override (override empty_valuation x true) y true);(override (override empty_valuation x false) y true)] z) [x;y;z]).
 
  Eval compute in (all_valuations (enum_valuation [x;y;z]) [x;y;z]).
-End Test''.
+End Test_enum_valuation.
 
 Fixpoint try_valuation (lv: list valuation) (p : form) : option valuation :=
   match lv with
@@ -164,13 +159,9 @@ Definition find_valuation (p : form) : option valuation :=
   let vals := (enum_valuation ids) in
   try_valuation vals p.
 
-Module Test'''.
+Module Test_find_valuation.
  Definition x := (var (Id "x")).
  Definition y := (var (Id "y")).
-
- Check (land (lor x (not y)) (lor (not x) y) ).
- Check (mapsto (not y) (lor x y) ).
- Check (land (land x (not x)) (bool true)).
 
  Definition apply_test (ov : option valuation) (i :id) :option Datatypes.bool :=
    match ov with
@@ -178,7 +169,7 @@ Module Test'''.
    |None => None
    end.
 
- Fixpoint apply_list  (ov : option valuation) (l :list id) : list (option Datatypes.bool):=
+Fixpoint apply_list  (ov : option valuation) (l :list id) : list (option Datatypes.bool):=
    match l with 
    |nil => []
    | x :: xs => (apply_test ov x) :: (apply_list ov xs)
@@ -191,4 +182,217 @@ Definition find_valuation' (p : form) : list (option Datatypes.bool) :=
  
  Eval compute in (find_valuation' (land (land x (not x)) (bool true))). 
 
-End Test'''.                              
+End Test_find_valuation.
+
+
+Definition solver (p : form) :Datatypes.bool:=
+  match find_valuation p with
+  | Some _ => true
+  | None => false
+  end.
+
+
+Lemma and_interp: forall p1 p2 V, interp V p1=true /\ interp V p2=true <-> interp V (land p1 p2)=true.
+Proof.
+  intros.
+  split.
+  - intro.
+    destruct H.
+     unfold interp.
+     unfold interp in H,H0.
+     now rewrite H,H0.
+  - intro.
+    split;
+
+    unfold interp in H;
+      symmetry in  H;
+      apply Bool.andb_true_eq in H;
+      destruct H;
+      unfold interp;
+      symmetry;
+      assumption.
+      
+Qed.
+
+(*
+Lemma find_val_rec : forall p v v' l, interp v p = true \/ (interp v p = false /\ try_valuation l p= Some v' ) ->  (exists V, try_valuation (v::l) p=Some V).
+Proof.
+  intros.
+  destruct H.
+  - exists v.
+    unfold try_valuation.
+    now rewrite H.
+  - exists v'.
+    unfold try_valuation.
+    destruct H.
+    rewrite H.
+    unfold try_valuation in H0.
+    assumption.
+Qed.
+
+
+Lemma try_val_rec : forall p v l, try_valuation (v::l) p = Some v \/ try_valuation (v::l) p = try_valuation l p .
+Proof.
+  intros.
+  unfold try_valuation.
+  destruct (interp v p) eqn:E.
+  - now left.
+  - now right.
+Qed.
+  
+
+Lemma and_solver: forall p1 p2 V, find_valuation (land p1 p2)=Some V -> satisfiable p1.
+Proof.
+  intros.
+    unfold find_valuation in H.
+    unfold try_valuation in H.
+    induction (enum_valuation (collect_var (land p1 p2))). 
+    + discriminate H.
+    +  destruct (interp a (land p1 p2)) eqn: E1.
+       * unfold satisfiable.
+         exists a.
+         apply and_interp in E1.
+         destruct E1.
+         assumption.
+       * apply IHl. (*why it works?*)
+         apply H.
+Qed.*)
+
+Lemma and_solver': forall p1 p2 V, find_valuation (land p1 p2)=Some V -> interp V p1=true /\ interp V p2=true.
+Proof.
+  intros.
+  split;unfold find_valuation in H;
+    unfold try_valuation in H;
+    induction (enum_valuation (collect_var (land p1 p2)));
+    try(discriminate H);
+    try(  destruct (interp a (land p1 p2)) eqn: E1);
+    
+       try(inversion H;
+         apply and_interp in E1;
+         destruct E1;
+         rewrite <-H1;
+         assumption);
+       try(apply IHl; (*why it works?*)
+         apply H).
+Qed.
+
+Lemma or_interp: forall p1 p2 V, interp V p1=true \/ interp V p2=true <-> interp V (lor p1 p2)=true.
+Proof.
+  intros.
+  split.
+  - intro.
+    destruct H.
+     unfold interp.
+     unfold interp in H.
+     rewrite H. reflexivity.
+     unfold interp.
+     unfold interp in H.
+     rewrite H. Search orb. apply Bool.orb_true_r.
+  - intro.
+
+    unfold interp in H.
+    Search orb.
+    apply Bool.orb_prop in H.
+   
+      unfold interp;
+      assumption.
+      
+Qed.
+
+
+Lemma or_solver': forall p1 p2 V, find_valuation (lor p1 p2)=Some V -> interp V p1=true \/ interp V p2=true.
+Proof.
+  intros.
+  unfold find_valuation in H;
+    unfold try_valuation in H;
+    induction (enum_valuation (collect_var (lor p1 p2))).
+    - discriminate H.
+    - destruct (interp a (lor p1 p2)) eqn: E1.
+    
+       + inversion H.
+         apply or_interp in E1.
+         rewrite <-H1;
+           assumption.
+         
+     +   try(apply IHl; (*why it works?*)
+         apply H).
+Qed.
+
+
+(*
+Lemma test:forall (A B:Prop) (H1:A/\ B -> exists A, A-> B) (H2: A /\ B), A\/B.
+Proof.
+  intros.
+  apply H1 in H2.
+  
+  assumption.
+Qed. 
+*) 
+(*
+Lemma and_satisfiable : forall p1 p2, satisfiable p1 -> satisfiable p2 -> satisfiable (land p1 p2).
+Proof.
+  intros.
+  unfold satisfiable in H, H0.
+  unfold satisfiable.
+  setoid_rewrite  <-and_interp.
+  destruct H,H0.
+  
+didn't work because the lemma is false!
+*)
+  
+  
+  
+  
+Lemma solver_sound : forall p, solver p = true -> satisfiable p.
+Proof.
+  intros.
+  induction p.
+  - unfold satisfiable.
+    exists (override empty_valuation i true).
+    simpl.
+    unfold override.
+    now rewrite  <- beq_id_refl.
+  - unfold solver in H.
+    destruct (find_valuation (bool b)) eqn:E in H .
+    +  unfold find_valuation in E.
+       
+       simpl in E.
+       
+       destruct b.
+       
+       unfold satisfiable.       
+       now exists v.
+                  discriminate  E.
+                  +  discriminate H.
+                  -  (*land*)
+                    unfold satisfiable.
+                    
+                    unfold solver in H.
+                    destruct (find_valuation (land p1 p2)) eqn:E in H .
+                    +  
+                    exists v.
+                    apply and_interp.
+                    apply and_solver' in E.
+                    assumption.
+                  +
+                    discriminate H.
+
+                  - (*lor*)
+                    unfold satisfiable.
+                    
+                    unfold solver in H.
+                    destruct (find_valuation (lor p1 p2)) eqn:E in H .
+                    + exists v.
+                      apply or_interp.
+                      apply or_solver' in E.
+                      assumption.
+                    +  discriminate H.
+                    -  Admitted. (*TODO: mapsto*)   
+                    
+                  
+                  
+
+    
+    
+     
+  
